add prototype of frontend

refinedVST/typing/frontend_stuff/examples/test_f_temps.c
@@ -8,6 +8,5 @@ int main() {
 [[rc::ensures("{n = 42}")]]
 int f_temps() {
     int a = 1;
-    int b = 41;
-    return a + b;
+    return a + 41;
 }
