RefinedVST.md
@@ -1,0 +1,34 @@
+# RefinedVST
+The refinedVST project is adapted from [RefinedC](https://gitlab.mpi-sws.org/iris/refinedc/-/commits/ea6be6de7f27855a79c9ca18e6a54ba3bd5ed883).
+
+This is still work in progress.
+
+## Build Instruction
+We will need VST, RefinedC (and for now, compcert (3.13 or 3.14) to generate the frontend). We assume the dependency of VST is installed and an opam switch is set up.
+
+TODO fix VST build instruction
+
+### VST
+The interface of the backend of RefinedVST is refinedVST/typing/typing.v:
+```
+make refinedVST/typing/typing.vo -j <jobs>
+```
+
+### RefinedC
+RefinedC: VST is pinned to a slightly older version of Iris (dev.2024-03-12.0.c1e15cdc), and consequently a slightly older version of [RefinedC dev.2024-07-23.0.ea6be6de](https://gitlab.mpi-sws.org/iris/refinedc/-/tree/ea6be6de7f27855a79c9ca18e6a54ba3bd5ed883).
+I failed to pin RefinedC's gitlab repository, but installing it from source works:
+```
+git clone https://gitlab.mpi-sws.org/iris/refinedc.git refinedc
+cd refinedc
+git branch pin_refinedc ea6be6de
+opam pin add refinedc . -y
+```
+
+## Running the frontend
+The entry point for the frontend is in [./refinedVST/typing/frontend_stuff/Makefile](./refinedVST/typing/frontend_stuff/Makefile), adapted from the RefinedC frontend.
+
+However the best way to use the frontend is to use the script [RefinedVST.sh](RefinedVST.sh):
+```
+./RefinedVST.sh
+```
+ The script checks [./refinedVST/typing/frontend_stuff/examples/test_f_temps.c](./refinedVST/typing/frontend_stuff/examples/test_f_temps.c) and generates proofs in [./refinedVST/typing/frontend_stuff/examples/proofs](./refinedVST/typing/frontend_stuff/examples/proofs).
